Use Comparse tactic

fstar/MLS.NetworkBinder.fst
@@ -8,61 +8,31 @@ open MLS.Tree
 module TS = MLS.TreeSync.Types
 module TK = MLS.TreeKEM.Types
 
-val network_to_option: #a:Type -> option_nt a -> result (option a)
-let network_to_option #a opt =
-  match opt with
-  | None_nt -> return None
-  | Some_nt x -> return (Some x)
-  | _ -> error "network_to_option: not a valid option"
-
-val option_to_network: #a:Type -> option a -> option_nt a
-let option_to_network #a opt =
-  match opt with
-  | None -> None_nt
-  | Some x -> Some_nt x
-
-
 noeq type leaf_package_content_nt (bytes:Type0) {|bytes_like bytes|} = {
   public_key: hpke_public_key_nt bytes;
 }
 
-val ps_leaf_package_content: #bytes:Type0 -> {|bytes_like bytes|} -> parser_serializer bytes (leaf_package_content_nt bytes)
-let ps_leaf_package_content #bytes #bl =
-  mk_isomorphism (leaf_package_content_nt bytes)
-    ps_hpke_public_key
-    (fun public_key -> ({public_key = public_key}))
-    (fun x -> x.public_key)
+%splice [ps_leaf_package_content_nt] (gen_parser (`leaf_package_content_nt))
 
 instance parseable_serializeable_leaf_package_content_nt (bytes:Type0) {|bytes_like bytes|}: parseable_serializeable bytes (leaf_package_content_nt bytes) =
-  mk_parseable_serializeable ps_leaf_package_content
+  mk_parseable_serializeable ps_leaf_package_content_nt
 
 noeq type node_package_content_nt (bytes:Type0) {|bytes_like bytes|} = {
   public_key: hpke_public_key_nt bytes;
-  encrypted_path_secret: blseq (hpke_ciphertext_nt bytes) ps_hpke_ciphertext ({min=0; max=(pow2 32)-1});
+  encrypted_path_secret: blseq bytes ps_hpke_ciphertext_nt ({min=0; max=(pow2 32)-1});
   last_group_context: blbytes bytes ({min=0; max=(pow2 64) - 1});
 }
 
-val ps_node_package_content: #bytes:Type0 -> {|bytes_like bytes|} -> parser_serializer bytes (node_package_content_nt bytes)
-let ps_node_package_content #bytes #bl =
-  let open Comparse in
-  mk_isomorphism (node_package_content_nt bytes)
-    (
-      _ <-- ps_hpke_public_key;
-      bind (ps_blseq _ ps_hpke_ciphertext) (fun (_:blseq (hpke_ciphertext_nt bytes) ps_hpke_ciphertext ({min=0; max=(pow2 32)-1})) -> //See FStarLang/FStar#2589
-      ps_blbytes _
-      )
-    )
-    (fun (|public_key, (|encrypted_path_secret, last_group_context|)|) -> ({public_key = public_key; encrypted_path_secret = encrypted_path_secret; last_group_context = last_group_context;}))
-    (fun x -> (|x.public_key, (|x.encrypted_path_secret, x.last_group_context|)|))
+%splice [ps_node_package_content_nt] (gen_parser (`node_package_content_nt))
 
 instance parseable_serializeable_node_package_content_nt (bytes:Type0) {|bytes_like bytes|}: parseable_serializeable bytes (node_package_content_nt bytes) =
-  mk_parseable_serializeable ps_node_package_content
+  mk_parseable_serializeable ps_node_package_content_nt
 
 (*** NetworkTreeSyncBinder ***)
 
 val key_package_to_treesync: #bytes:Type0 -> {|bytes_like bytes|} -> key_package_nt bytes -> result (TS.leaf_package_t bytes)
 let key_package_to_treesync #bytes #bl kp =
-  match kp.credential with
+  match kp.tbs.credential with
   | C_basic cred ->
     return ({
       TS.credential = {
@@ -70,10 +40,10 @@ let key_package_to_treesync #bytes #bl kp =
         TS.identity = cred.identity;
         TS.signature_key = cred.signature_key;
       };
-      TS.endpoint_id = kp.endpoint_id;
+      TS.endpoint_id = kp.tbs.endpoint_id;
       TS.version = 0;
-      TS.content = serialize (leaf_package_content_nt bytes) ({public_key = kp.public_key});
-      TS.extensions = (ps_to_pse (ps_blseq _ ps_extension)).serialize_exact (kp.extensions);
+      TS.content = serialize (leaf_package_content_nt bytes) ({public_key = kp.tbs.public_key});
+      TS.extensions = (ps_to_pse (ps_blseq ps_extension_nt _)).serialize_exact (kp.tbs.extensions);
       TS.signature = kp.signature;
     })
   | _ -> error "key_package_to_treesync: credential type not supported"
@@ -89,20 +59,22 @@ let treesync_to_keypackage #bytes #cb lp =
   else if not (length lp.TS.signature < pow2 16) then
     error "treesync_to_keypackage: signature too long"
   else (
-    leaf_content <-- from_option "treesync_to_keypackage: can't parse leaf content" ((ps_to_pse ps_leaf_package_content).parse_exact lp.TS.content);
-    extensions <-- from_option "treesync_to_keypackage: can't parse extensions" ((ps_to_pse (ps_blseq _ ps_extension)).parse_exact lp.TS.extensions);
+    leaf_content <-- from_option "treesync_to_keypackage: can't parse leaf content" (parse (leaf_package_content_nt bytes) lp.TS.content);
+    extensions <-- from_option "treesync_to_keypackage: can't parse extensions" ((ps_to_pse (ps_blseq ps_extension_nt _)).parse_exact lp.TS.extensions);
     let cipher_suite = available_ciphersuite_to_network (ciphersuite #bytes) in
     return ({
-      version = PV_mls10;
-      cipher_suite = cipher_suite;
-      public_key = leaf_content.public_key;
-      endpoint_id = lp.TS.endpoint_id;
-      credential = C_basic ({
-        identity = lp.TS.credential.TS.identity;
-        signature_scheme = SA_ed25519; //TODO
-        signature_key = lp.TS.credential.TS.signature_key;
-      });
-      extensions = extensions;
+      tbs = {
+        version = PV_mls10 ();
+        cipher_suite = cipher_suite;
+        public_key = leaf_content.public_key;
+        endpoint_id = lp.TS.endpoint_id;
+        credential = C_basic ({
+          identity = lp.TS.credential.TS.identity;
+          signature_scheme = SA_ed25519 (); //TODO
+          signature_key = lp.TS.credential.TS.signature_key;
+        });
+        extensions = extensions;
+      };
       signature = lp.TS.signature;
     } <: key_package_nt bytes)
   )
@@ -116,7 +88,7 @@ let treesync_to_parent_node #bytes #bl np =
     internal_failure "treesync_to_parent_node: unmerged_leaves too long"
   else (
     Seq.lemma_list_seq_bij unmerged_leaves;
-    node_content <-- from_option "treesync_to_parent_node: can't parse content" ((ps_to_pse ps_node_package_content).parse_exact np.TS.content);
+    node_content <-- from_option "treesync_to_parent_node: can't parse content" (parse (node_package_content_nt bytes) np.TS.content);
     return ({
       public_key = node_content.public_key;
       parent_hash = np.TS.parent_hash;
@@ -126,7 +98,7 @@ let treesync_to_parent_node #bytes #bl np =
 
 val parent_node_to_treesync: #bytes:Type0 -> {|bytes_like bytes|} -> parent_node_nt bytes -> result (TS.node_package_t bytes)
 let parent_node_to_treesync #bytes #bl pn =
-  bytes_length_nil #bytes ps_hpke_ciphertext;
+  bytes_length_nil #bytes ps_hpke_ciphertext_nt;
   return ({
         TS.version = 0;
         TS.content_dir = Left; //We don't care I guess
@@ -143,11 +115,11 @@ let parent_node_to_treesync #bytes #bl pn =
 //Refactor?
 val key_package_to_treekem: #bytes:Type0 -> {|crypto_bytes bytes|} -> key_package_nt bytes -> result (TK.member_info bytes)
 let key_package_to_treekem #bytes #cb kp =
-  if not (length (kp.public_key <: bytes) = hpke_public_key_length #bytes) then
+  if not (length (kp.tbs.public_key <: bytes) = hpke_public_key_length #bytes) then
     error "key_package_to_treekem: public key has wrong length"
   else
     return ({
-      TK.public_key = kp.public_key;
+      TK.public_key = kp.tbs.public_key;
       TK.version = 0;
     } <: TK.member_info bytes)
 
@@ -196,7 +168,7 @@ let rec update_path_to_treekem #bytes #cb l n i group_context update_path =
       let head_update_path_nodes = Seq.index update_path.nodes (update_path_length-1) in
       let tail_update_path_nodes = Seq.slice update_path.nodes 0 (update_path_length-1) in
       //TODO this is an easy lemma
-      assume (bytes_length ps_update_path_node (Seq.seq_to_list tail_update_path_nodes) <= bytes_length ps_update_path_node (Seq.seq_to_list update_path.nodes));
+      assume (bytes_length ps_update_path_node_nt (Seq.seq_to_list tail_update_path_nodes) <= bytes_length ps_update_path_node_nt (Seq.seq_to_list update_path.nodes));
       let next_update_path = { update_path with nodes = tail_update_path_nodes } in
       let (|dir, next_i|) = child_index l i in
       path_next <-- update_path_to_treekem (l-1) (if dir = Left then pow2 (l-1) else n - (pow2 (l-1))) next_i group_context next_update_path;
@@ -208,7 +180,7 @@ let rec update_path_to_treekem #bytes #cb l n i group_context update_path =
 
 val treesync_to_update_path_node: #bytes:Type0 -> {|bytes_like bytes|} -> TS.node_package_t bytes -> result (update_path_node_nt bytes)
 let treesync_to_update_path_node #bytes #bl np =
-  node_content <-- from_option "treesync_to_update_path_node: can't parse content" ((ps_to_pse ps_node_package_content).parse_exact np.TS.content);
+  node_content <-- from_option "treesync_to_update_path_node: can't parse content" (parse (node_package_content_nt bytes) np.TS.content);
   return ({
     public_key = node_content.public_key;
     encrypted_path_secret = node_content.encrypted_path_secret;
@@ -238,7 +210,7 @@ let treesync_to_update_path #bytes #cb #l #n #i p =
   let (kp, upns) = tmp in
   let upns = List.rev upns in
   Seq.lemma_list_seq_bij upns;
-  if not (bytes_length ps_update_path_node upns < pow2 32) then
+  if not (bytes_length ps_update_path_node_nt upns < pow2 32) then
     error "treesync_to_update_path: nodes too long"
   else
     return ({
@@ -265,18 +237,17 @@ let ratchet_tree_l_n #bytes #bl nodes =
     let l = (TreeMath.Internal.log2 n) + 1 in
     return (|l, n|)
 
-val ratchet_tree_to_treesync: #bytes:Type0 -> {|bytes_like bytes|} -> l:nat -> n:tree_size l -> nodes:Seq.seq (option_nt (node_nt bytes)){Seq.length nodes = (n+n-1)} -> result (TS.treesync bytes l n)
+val ratchet_tree_to_treesync: #bytes:Type0 -> {|bytes_like bytes|} -> l:nat -> n:tree_size l -> nodes:Seq.seq (option (node_nt bytes)){Seq.length nodes = (n+n-1)} -> result (TS.treesync bytes l n)
 let rec ratchet_tree_to_treesync #bytes #bl l n nodes =
   if l = 0 then (
     assert (Seq.length nodes == 1);
     match (Seq.index nodes 0) with
-    | Some_nt (N_leaf kp) ->
+    | Some (N_leaf kp) ->
       kp <-- key_package_to_treesync kp;
       return (TLeaf (dumb_credential, Some kp))
-    | Some_nt _ -> error "ratchet_tree_to_treesync_aux: node must be a leaf!"
-    | None_nt ->
+    | Some _ -> error "ratchet_tree_to_treesync_aux: node must be a leaf!"
+    | None ->
       return (TLeaf (dumb_credential, None))
-    | _ -> error "ratchet_tree_to_treesync_aux: option is invalid"
   ) else if n <= pow2 (l-1) then (
     res <-- ratchet_tree_to_treesync (l-1) n nodes;
     return (TSkip _ res)
@@ -287,32 +258,31 @@ let rec ratchet_tree_to_treesync #bytes #bl l n nodes =
     left_res <-- ratchet_tree_to_treesync (l-1) (pow2 (l-1)) left_nodes;
     right_res <-- ratchet_tree_to_treesync (l-1) (n-pow2 (l-1)) right_nodes;
     match my_node with
-    | Some_nt (N_parent pn) ->
+    | Some (N_parent pn) ->
       np <-- parent_node_to_treesync pn;
       return (TNode (dumb_credential, Some np) left_res right_res)
-    | Some_nt _ -> error "ratchet_tree_to_treesync_aux: node must be a parent!"
-    | None_nt ->
+    | Some _ -> error "ratchet_tree_to_treesync_aux: node must be a parent!"
+    | None ->
       return (TNode (dumb_credential, None) left_res right_res)
-    | _ -> error "ratchet_tree_to_treesync_aux: option is invalid"
   )
 
-val treesync_to_ratchet_tree: #bytes:Type0 -> {|crypto_bytes bytes|} -> #l:nat -> #n:tree_size l -> TS.treesync bytes l n -> result (Seq.seq (option_nt (node_nt bytes)))
+val treesync_to_ratchet_tree: #bytes:Type0 -> {|crypto_bytes bytes|} -> #l:nat -> #n:tree_size l -> TS.treesync bytes l n -> result (Seq.seq (option (node_nt bytes)))
 let rec treesync_to_ratchet_tree #bytes #cb #l #n t =
   match t with
   | TLeaf (_, None) ->
-    return (Seq.create 1 None_nt)
+    return (Seq.create 1 None)
   | TLeaf (_, Some lp) ->
     key_package <-- treesync_to_keypackage lp;
-    return (Seq.create 1 (Some_nt (N_leaf (key_package))))
+    return (Seq.create 1 (Some (N_leaf (key_package))))
   | TSkip _ t' ->
     treesync_to_ratchet_tree t'
   | TNode (_, onp) left right ->
     parent_node <-- (
       match onp with
-      | None -> return None_nt
+      | None -> return None
       | Some np ->
         result <-- treesync_to_parent_node np;
-        return (Some_nt (N_parent result))
+        return (Some (N_parent result))
     );
     left_ratchet <-- treesync_to_ratchet_tree left;
     right_ratchet <-- treesync_to_ratchet_tree right;
