fstar/MLS.TreeSync.Hash.fst
@@ -13,55 +13,27 @@ open MLS.Result
 
 noeq type leaf_node_tree_hash_input_nt (bytes:Type0) {|bytes_like bytes|} = {
   node_index: nat_lbytes 4;
-  key_package: option_nt (key_package_nt bytes);
+  [@@@ with_parser #bytes (ps_option ps_key_package_nt)]
+  key_package: option (key_package_nt bytes);
 }
 
-val ps_leaf_node_tree_hash_input: #bytes:Type0 -> {|bytes_like bytes|} -> parser_serializer bytes (leaf_node_tree_hash_input_nt bytes)
-let ps_leaf_node_tree_hash_input #bytes #bl =
-  let open Comparse in
-  mk_isomorphism (leaf_node_tree_hash_input_nt bytes)
-    (
-      _ <-- ps_nat_lbytes 4;
-      ps_option (ps_key_package)
-    )
-  (fun (|node_index, key_package|) -> {
-    node_index = node_index;
-    key_package = key_package;
-  })
-  (fun x -> (|x.node_index, x.key_package|))
+%splice [ps_leaf_node_tree_hash_input_nt] (gen_parser (`leaf_node_tree_hash_input_nt))
 
 instance parseable_serializeable_leaf_node_tree_hash_input (bytes:Type0) {|bytes_like bytes|}: parseable_serializeable bytes (leaf_node_tree_hash_input_nt bytes) =
-  mk_parseable_serializeable ps_leaf_node_tree_hash_input
+  mk_parseable_serializeable ps_leaf_node_tree_hash_input_nt
 
 noeq type parent_node_tree_hash_input_nt (bytes:Type0) {|bytes_like bytes|} = {
   node_index: nat_lbytes 4;
-  parent_node: option_nt (parent_node_nt bytes);
+  [@@@ with_parser #bytes (ps_option ps_parent_node_nt)]
+  parent_node: option (parent_node_nt bytes);
   left_hash: blbytes bytes ({min=0;max=255});
   right_hash: blbytes bytes ({min=0;max=255});
 }
 
-#push-options "--ifuel 2"
-val ps_parent_node_tree_hash_input: #bytes:Type0 -> {|bytes_like bytes|} -> parser_serializer bytes (parent_node_tree_hash_input_nt bytes)
-let ps_parent_node_tree_hash_input #bytes #bl =
-  let open Comparse in
-  mk_isomorphism (parent_node_tree_hash_input_nt bytes)
-    (
-      _ <-- ps_nat_lbytes 4;
-      _ <-- ps_option (ps_parent_node);
-      _ <-- ps_blbytes #bytes _; //See FStarLang/FStar#2583 for why the annotation
-      ps_blbytes _
-    )
-  (fun (|node_index, (|parent_node, (|left_hash, right_hash|)|)|) -> {
-    node_index = node_index;
-    parent_node = parent_node;
-    left_hash = left_hash;
-    right_hash = right_hash;
-  })
-  (fun x -> (|x.node_index, (|x.parent_node, (|x.left_hash, x.right_hash|)|)|))
-#pop-options
+%splice [ps_parent_node_tree_hash_input_nt] (gen_parser (`parent_node_tree_hash_input_nt))
 
 instance parseable_serializeable_parent_node_tree_hash_input (bytes:Type0) {|bytes_like bytes|}: parseable_serializeable bytes (parent_node_tree_hash_input_nt bytes) =
-  mk_parseable_serializeable ps_parent_node_tree_hash_input
+  mk_parseable_serializeable ps_parent_node_tree_hash_input_nt
 
 val tree_hash: #bytes:Type0 -> {|crypto_bytes bytes|} -> #l:nat -> #n:tree_size l -> TM.node_index l -> treesync bytes l n -> result (lbytes bytes (hash_length #bytes))
 let rec tree_hash #bytes #cb #l #n ind t =
@@ -70,10 +42,10 @@ let rec tree_hash #bytes #cb #l #n ind t =
   | TLeaf (_, olp) ->
     key_package <-- (
       match olp with
-      | None -> return None_nt
+      | None -> return None
       | Some lp ->
         res <-- treesync_to_keypackage lp;
-        return (Some_nt res)
+        return (Some res)
     );
     if not (ind < pow2 32) then
       internal_failure "tree_hash: node_index too big"
@@ -85,10 +57,10 @@ let rec tree_hash #bytes #cb #l #n ind t =
   | TNode (_, onp) left right ->
     parent_node <-- (
       match onp with
-      | None -> return None_nt
+      | None -> return None
       | Some np ->
         res <-- treesync_to_parent_node np;
-        return (Some_nt res)
+        return (Some res)
     );
     left_hash <-- tree_hash (TM.left ind) left;
     right_hash <-- tree_hash (TM.right ind) right;
